Lang_Untyped.thy
@@ -84,19 +84,20 @@ lemma fresh_variables_local_type: "map vu_type (fresh_variables_local used ts) =
 
 subsection {* Memories *}
 
-
+(*
 record memory_rep = 
   mem_globals :: "variable_untyped \<Rightarrow> val"
   mem_locals :: "variable_untyped \<Rightarrow> val"
 (*  mem_stack :: "(variable_untyped \<Rightarrow> val) list" *)
+*)
 
-typedef memory = "{m::memory_rep. 
-     (\<forall>v. mem_globals m v \<in> t_domain (vu_type v))
-   \<and> (\<forall>v. mem_locals m v \<in> t_domain (vu_type v))
-(*   \<and> (\<forall>s\<in>set (mem_stack m). \<forall>v. s v \<in> t_domain (vu_type v))*)}"
-apply (rule exI[where x="\<lparr> mem_globals = (\<lambda>v. t_default (vu_type v)),
+typedef memory = "{m::variable_untyped \<Rightarrow> val. (\<forall>v. m v \<in> t_domain (vu_type v))}"
+  by (rule exI[of _ "(\<lambda>v. t_default (vu_type v))"], simp)
+(*   \<and> (\<forall>v. mem_locals m v \<in> t_domain (vu_type v))e ve
+(*   \<and> (\<forall>s\<in>set (mem_stack m). \<forall>v. s v \<in> t_domain (vu_type v))*)}"*)
+(*apply (rule exI[where x="\<lparr> mem_globals = (\<lambda>v. t_default (vu_type v)),
                            mem_locals = (\<lambda>v. t_default (vu_type v)) \<rparr>"])
-  by auto
+  by auto*)
 
 (*
 typedef memory = "{(m::variable_untyped\<Rightarrow>val). (\<forall>v. m v \<in> t_domain (vu_type v))}"
